Renamed files for BST and RBT.

HOL/DataStrs/BST.thy
@@ -1,7 +1,6 @@
-(* Base of binary search trees, to be used in verification of both
-   functional and imperative programs. *)
+(* Verification of functional programs on binary search trees. *)
 
-theory BST_Base
+theory BST
 imports Lists_Ex
 begin
 
@@ -81,5 +80,80 @@ lemma rotateR_in_trav [rewrite]: "in_traverse (rotateR t) = in_traverse t" by au
 
 lemma rotateL_sorted [forward]: "tree_sorted t \<Longrightarrow> tree_sorted (rotateL t)" by auto2
 lemma rotateR_sorted [forward]: "tree_sorted t \<Longrightarrow> tree_sorted (rotateR t)" by auto2
+
+section {* Insertion on trees *}
+
+fun tree_insert :: "'a::ord \<Rightarrow> 'b \<Rightarrow> ('a, 'b) tree \<Rightarrow> ('a, 'b) tree" where
+  "tree_insert x v Tip = Node Tip x v Tip"
+| "tree_insert x v (Node l y w r) =
+    (if x = y then Node l x v r
+     else if x < y then Node (tree_insert x v l) y w r
+     else Node l y w (tree_insert x v r))"
+setup {* fold add_rewrite_rule @{thms tree_insert.simps} *}
+ 
+lemma insert_in_traverse_pairs [rewrite]:
+  "tree_sorted t \<Longrightarrow> in_traverse_pairs (tree_insert x v t) = ordered_insert_pairs x v (in_traverse_pairs t)"
+@proof @induct t @qed
+
+theorem insert_sorted [forward]:
+  "tree_sorted t \<Longrightarrow> tree_sorted (tree_insert x v t)" by auto2
+
+theorem insert_on_map:
+  "tree_sorted t \<Longrightarrow> tree_map (tree_insert x v t) = (tree_map t) {x \<rightarrow> v}" by auto2
+
+section {* Deletion on trees *}
+
+fun del_min :: "('a, 'b) tree \<Rightarrow> ('a \<times> 'b) \<times> ('a, 'b) tree" where
+  "del_min Tip = undefined"
+| "del_min (Node lt x v rt) =
+   (if lt = Tip then ((x, v), rt) else
+    (fst (del_min lt), Node (snd (del_min lt)) x v rt))"
+setup {* add_rewrite_rule @{thm del_min.simps(2)} *}
+
+lemma delete_min_del_hd_pairs [rewrite]:
+  "t \<noteq> Tip \<Longrightarrow> fst (del_min t) # in_traverse_pairs (snd (del_min t)) = in_traverse_pairs t"
+@proof @induct t @qed
+
+fun delete_elt_tree :: "('a, 'b) tree \<Rightarrow> ('a, 'b) tree" where
+  "delete_elt_tree Tip = undefined"
+| "delete_elt_tree (Node lt x v rt) =
+    (if lt = Tip then rt else if rt = Tip then lt else
+     Node lt (fst (fst (del_min rt))) (snd (fst (del_min rt))) (snd (del_min rt)))"
+setup {* add_rewrite_rule @{thm delete_elt_tree.simps(2)} *}
+
+lemma delete_elt_in_traverse_pairs [rewrite]:
+  "in_traverse_pairs (delete_elt_tree (Node lt x v rt)) = in_traverse_pairs lt @ in_traverse_pairs rt" by auto2
+
+fun tree_delete :: "'a::ord \<Rightarrow> ('a, 'b) tree \<Rightarrow> ('a, 'b) tree" where
+  "tree_delete x Tip = Tip"
+| "tree_delete x (Node l y w r) =
+    (if x = y then delete_elt_tree (Node l y w r)
+     else if x < y then Node (tree_delete x l) y w r
+     else Node l y w (tree_delete x r))"
+setup {* fold add_rewrite_rule @{thms tree_delete.simps} *}
+
+lemma tree_delete_in_traverse_pairs [rewrite]:
+  "tree_sorted t \<Longrightarrow> in_traverse_pairs (tree_delete x t) = remove_elt_pairs x (in_traverse_pairs t)"
+@proof @induct t @qed
+
+theorem tree_delete_sorted [forward]:
+  "tree_sorted t \<Longrightarrow> tree_sorted (tree_delete x t)" by auto2
+
+theorem tree_delete_map [rewrite]:
+  "tree_sorted t \<Longrightarrow> tree_map (tree_delete x t) = delete_map x (tree_map t)" by auto2
+
+section {* Search on sorted trees *}
+
+fun tree_search :: "('a::ord, 'b) tree \<Rightarrow> 'a \<Rightarrow> 'b option" where
+  "tree_search Tip x = None"
+| "tree_search (Node l k v r) x =
+  (if x = k then Some v
+   else if x < k then tree_search l x
+   else tree_search r x)"
+setup {* fold add_rewrite_rule @{thms tree_search.simps} *}
+
+theorem tree_search_correct [rewrite]:
+  "tree_sorted t \<Longrightarrow> tree_search t x = (tree_map t)\<langle>x\<rangle>"
+@proof @induct t @qed
 
 end
